reactive-angelic-designs/utp_rad_examples.thy
@@ -1,18 +1,25 @@
 section \<open>Reactive Angelic Design Examples\<close>
 
 text \<open>
-  The worked examples of the paper's Section 6.4 (Examples 15--17 and
-  Lemmas 8--9), collected apart from the operator theories.
+  The worked examples of the paper's Section 6 (Examples 11--21 and
+  Lemmas 5, 8, and 9), collected apart from the operator theories.
 \<close>
 
 theory utp_rad_examples
-  imports utp_rad_seq
+  imports utp_rad_nd
 begin
+
+subsection \<open>RA1 and PBMH do not commute (Example 11)\<close>
+
+(* Paper Example 11: the two compositions disagree on ac = {}. *)
+lemma RA1_PBMH_ades_ac_empty_example:
+  "RA1 (PBMH_ades rad_ac_empty) = RA1 true \<and>
+   PBMH_ades (RA1 rad_ac_empty) = false"
+  by (simp only: RA1_PBMH_ades_ac_empty PBMH_ades_RA1_ac_empty)
 
 subsection \<open>Angelic choice of Stop and Skip (Example 15, Lemma 8)\<close>
 
-(* Paper Example 15 / Thesis Example 32: the angelic choice between
-   deadlock and termination is not resolved in favour of either. *)
+(* Paper Example 15 / Thesis Example 32: stop \<squnion> skip *)
 lemma Stop_Skip_angelic_choice:
   "Stop\<^sub>R\<^sub>A\<^sub>D \<squnion>\<^sub>R\<^sub>A\<^sub>D Skip\<^sub>R\<^sub>A\<^sub>D =
    (RA \<circ> A) (true \<turnstile> (stop_post \<and> skip_post))"
@@ -181,7 +188,8 @@ lemma prefix_continuation_stop:
       RA2 (RA1 stop_post))) = prefix_stop_post a"
   apply (simp only: RA1_RA2_commute'[symmetric] RA2_stop_post)
   apply (simp add: RA1_def aseq_ades_def prefix_post_def stop_post_def
-      prefix_stop_post_def ades_state_choice_def expr_if_def
+      prefix_stop_post_def ades_singleton_choice_def
+      ades_state_choice_def expr_if_def
       rad_trace_extensions_def fun_eq_iff Let_def
       lens_defs rad_state.wait_def astate.s_def des_vars.more\<^sub>L_def
       bex_nonempty_absorb)
@@ -548,6 +556,508 @@ proof -
   also have "... = (a \<rightarrow>\<^sub>R\<^sub>A\<^sub>D Skip\<^sub>R\<^sub>A\<^sub>D)"
     by (simp only: Prefix_Skip_RAD_RA skip_absorb[symmetric])
   finally show ?thesis .
+qed
+
+
+subsection \<open>Different prefixed deadlocks (Example 12)\<close>
+
+(* Paper Example 12: both prefixed deadlocks must agree on a final state. *)
+lemma Prefix_Stop_Stop_angelic_choice:
+  "(a \<rightarrow>\<^sub>R\<^sub>A\<^sub>D Stop\<^sub>R\<^sub>A\<^sub>D) \<squnion>\<^sub>R\<^sub>A\<^sub>D (b \<rightarrow>\<^sub>R\<^sub>A\<^sub>D Stop\<^sub>R\<^sub>A\<^sub>D) =
+   (RA \<circ> A) (true \<turnstile> (prefix_stop_post a \<and> prefix_stop_post b))"
+proof -
+  have absorb_a:
+      "(RA \<circ> A) (true \<turnstile> prefix_stop_post a) =
+       RA (true \<turnstile> prefix_stop_post a)"
+    by (rule RA_A_absorb_design_true; simp add: Healthy_def' unrest)
+  have absorb_b:
+      "(RA \<circ> A) (true \<turnstile> prefix_stop_post b) =
+       RA (true \<turnstile> prefix_stop_post b)"
+    by (rule RA_A_absorb_design_true; simp add: Healthy_def' unrest)
+  have "(a \<rightarrow>\<^sub>R\<^sub>A\<^sub>D Stop\<^sub>R\<^sub>A\<^sub>D) \<squnion>\<^sub>R\<^sub>A\<^sub>D
+        (b \<rightarrow>\<^sub>R\<^sub>A\<^sub>D Stop\<^sub>R\<^sub>A\<^sub>D) =
+        (RA \<circ> A) (true \<turnstile> prefix_stop_post a) \<squnion>\<^sub>R\<^sub>A\<^sub>D
+        (RA \<circ> A) (true \<turnstile> prefix_stop_post b)"
+    by (simp only: Prefix_Stop_RAD_RA absorb_a absorb_b)
+  also have "... = (RA \<circ> A)
+      ((true \<turnstile> prefix_stop_post a) \<squnion>\<^sub>R\<^sub>A\<^sub>D
+       (true \<turnstile> prefix_stop_post b))"
+    apply (rule RA_A_angelic_choice)
+       apply (simp add: Healthy_def' design_as_disj PBMH_ades_disj
+          PBMH_ades_conj_ok)
+      apply (simp add: Healthy_def' design_as_disj PBMH_ades_disj
+          PBMH_ades_conj_ok)
+     apply (rule design_is_H1_H2; simp add: unrest)
+    by (rule design_is_H1_H2; simp add: unrest)
+  also have "... = (RA \<circ> A)
+      (true \<turnstile> (prefix_stop_post a \<and> prefix_stop_post b))"
+    apply (rule arg_cong[where f="RA \<circ> A"])
+    apply (simp only: design_inf)
+    by pred_auto
+  finally show ?thesis .
+qed
+
+
+subsection \<open>CSP agreement of different prefixed deadlocks (Lemma 5)\<close>
+
+(* Thesis Lemma L.A.3.3 normal form of CSP prefix followed by Stop. *)
+definition Prefix_Stop_R :: "'e \<Rightarrow> ('e list, 'e set) rp_hrel"
+  ("_ \<rightarrow>\<^sub>R Stop\<^sub>R" [81] 80) where
+[pred]: "a \<rightarrow>\<^sub>R Stop\<^sub>R = \<^bold>R (true \<turnstile> (\<lambda> (s, y).
+  rea_vars.wait\<^sub>v y \<and>
+  (rea_vars.tr\<^sub>v y = rea_vars.tr\<^sub>v s \<and>
+     a \<notin> rea_vars.more y \<or>
+   rea_vars.tr\<^sub>v y = rea_vars.tr\<^sub>v s @ [a])))"
+
+definition csp_prefix_stop_pair_post ::
+  "'e \<Rightarrow> 'e \<Rightarrow> ('e list, 'e set) rp_hrel" where
+[pred]: "csp_prefix_stop_pair_post a b = (\<lambda> (s, y).
+  rea_vars.tr\<^sub>v y = rea_vars.tr\<^sub>v s \<and>
+  a \<notin> rea_vars.more y \<and> b \<notin> rea_vars.more y \<and>
+  rea_vars.wait\<^sub>v y)"
+
+(* Paper Lemma 5. The distinctness premise rules out agreement after an event. *)
+lemma Prefix_Stop_Stop_R:
+  fixes a b :: 'e
+  assumes "a \<noteq> b"
+  shows "(a \<rightarrow>\<^sub>R Stop\<^sub>R) \<squnion>
+      (b \<rightarrow>\<^sub>R Stop\<^sub>R) =
+    \<^bold>R (true \<turnstile> csp_prefix_stop_pair_post a b)"
+proof -
+  have R3c_conj:
+      "R3c (P \<and> Q) = (R3c P \<and> R3c Q)"
+      for P Q :: "('e list, 'e set) rp_hrel"
+    by pred_auto
+  have R2c_conj:
+      "R2c (P \<and> Q) = (R2c P \<and> R2c Q)"
+      for P Q :: "('e list, 'e set) rp_hrel"
+    by pred_auto
+  have RH_choice:
+      "\<^bold>R P \<squnion> \<^bold>R Q = \<^bold>R (P \<squnion> Q)"
+      for P Q :: "('e list, 'e set) rp_hrel"
+    by (simp only: conj_pred_def[symmetric];
+        simp add: RH_def R1_conj R2c_conj R3c_conj)
+  show ?thesis
+    apply (simp only: Prefix_Stop_R_def RH_choice)
+    apply (rule arg_cong[where f=RH])
+    apply (simp only: design_inf)
+    apply (simp add: csp_prefix_stop_pair_post_def fun_eq_iff)
+    using assms
+    by (pred_auto; auto)
+qed
+
+
+subsection \<open>Removing divergence (Examples 20-21)\<close>
+
+(* Paper Example 20. *)
+lemma NDRAD_Chaos_example:
+  "NDRAD Chaos\<^sub>R\<^sub>A\<^sub>D = Choice\<^sub>R\<^sub>A\<^sub>D"
+  by (rule NDRAD_Chaos)
+
+(* Paper Example 21. *)
+lemma NDRAD_Prefix_Skip:
+  "NDRAD (a \<rightarrow>\<^sub>R\<^sub>A\<^sub>D Skip\<^sub>R\<^sub>A\<^sub>D) =
+   (a \<rightarrow>\<^sub>R\<^sub>A\<^sub>D Skip\<^sub>R\<^sub>A\<^sub>D)"
+proof -
+  have choice_absorb:
+      "(RA \<circ> A) (true \<turnstile> true) = RA (true \<turnstile> true)"
+    by (rule RA_A_absorb_design_true[OF true_PBMH_ades];
+        simp add: unrest)
+  have design_absorb:
+      "((true \<turnstile> prefix_post a) \<and> (true \<turnstile> true)) =
+       (true \<turnstile> prefix_post a)"
+    by (simp add: design_def fun_eq_iff; pred_auto)
+  have "NDRAD (a \<rightarrow>\<^sub>R\<^sub>A\<^sub>D Skip\<^sub>R\<^sub>A\<^sub>D) =
+      (RA (true \<turnstile> prefix_post a) \<and>
+       RA (true \<turnstile> true))"
+    by (simp only: NDRAD_def RAD_angelic_choice Prefix_Skip_RAD_RA
+        Choice_RAD_alt choice_absorb)
+  also have "... = RA
+      ((true \<turnstile> prefix_post a) \<and> (true \<turnstile> true))"
+    by (simp only: RA_conj)
+  also have "... = RA (true \<turnstile> prefix_post a)"
+    by (simp only: design_absorb)
+  finally show ?thesis
+    by (simp only: Prefix_Skip_RAD_RA)
+qed
+
+
+subsection \<open>Different prefixed events (Example 18)\<close>
+
+lemma Prefix_Choice_RAD_RA:
+  "(a \<rightarrow>\<^sub>R\<^sub>A\<^sub>D Choice\<^sub>R\<^sub>A\<^sub>D) =
+   RA (true \<turnstile>
+       (prefix_offer_post a \<or> prefix_diverge_post a))"
+proof -
+  have component_unrests:
+      "$ok\<^sup>> \<sharp> (true :: ('e list, 'e) reactive_angelic_design)"
+      "$ok\<^sup>> \<sharp> prefix_post a"
+      "$ok\<^sup>< \<sharp> (true :: ('e list, 'e) reactive_angelic_design)"
+      "$ok\<^sup>< \<sharp> (true :: ('e list, 'e) reactive_angelic_design)"
+    by (simp_all add: unrest)
+  have not_true_PBMH:
+      "(\<not> (true :: ('e list, 'e) reactive_angelic_design)) is PBMH_ades"
+    by (simp only: pred_ba.compl_top_eq false_PBMH_ades)
+  have prefix_PBMH: "prefix_post a is PBMH_ades"
+    by (simp add: Healthy_def')
+  have choice_absorb:
+      "(RA \<circ> A) (true \<turnstile> true) = RA (true \<turnstile> true)"
+    by (rule RA_A_absorb_design_true[OF true_PBMH_ades]; simp add: unrest)
+  have "(a \<rightarrow>\<^sub>R\<^sub>A\<^sub>D Choice\<^sub>R\<^sub>A\<^sub>D) =
+      (RA (true \<turnstile> prefix_post a) ;;\<^sub>D\<^sub>A
+       RA (true \<turnstile> true))"
+    by (simp only: Prefix_RAD_def PrefixSkip_RAD_RA Choice_RAD_alt
+        choice_absorb)
+  also have "... = RA (true \<turnstile>
+      (prefix_offer_post a \<or> prefix_diverge_post a))"
+    using RA_design_seq[
+      where P=true and Q="prefix_post a" and R=true and S=true,
+      OF component_unrests not_true_PBMH prefix_PBMH]
+    by (simp only: pred_ba.compl_top_eq pred_ba.compl_bot_eq
+        pred_impl_laws RA1_false RA2_false aseq_ades_false_left
+        pred_ba.inf_bot_right RA1_aseq_false prefix_continuation_chaos
+        pred_ba.inf_top_left)
+  finally show ?thesis .
+qed
+
+
+(* Paper Example 18: divergence after b is replaced by non-divergent choice. *)
+lemma Prefix_Skip_Chaos_different_events:
+  assumes "a \<noteq> b"
+  shows "(a \<rightarrow>\<^sub>R\<^sub>A\<^sub>D Skip\<^sub>R\<^sub>A\<^sub>D) \<squnion>\<^sub>R\<^sub>A\<^sub>D
+    (b \<rightarrow>\<^sub>R\<^sub>A\<^sub>D Chaos\<^sub>R\<^sub>A\<^sub>D) =
+    (a \<rightarrow>\<^sub>R\<^sub>A\<^sub>D Skip\<^sub>R\<^sub>A\<^sub>D) \<squnion>\<^sub>R\<^sub>A\<^sub>D
+    (b \<rightarrow>\<^sub>R\<^sub>A\<^sub>D Choice\<^sub>R\<^sub>A\<^sub>D)"
+proof -
+  have design_eq:
+      "((true \<turnstile> prefix_post a) \<and>
+        ((\<not> prefix_diverge_post b) \<turnstile>
+          (prefix_offer_post b \<or> prefix_diverge_post b))) =
+       ((true \<turnstile> prefix_post a) \<and>
+        (true \<turnstile>
+          (prefix_offer_post b \<or> prefix_diverge_post b)))"
+    apply (simp add: prefix_post_def prefix_offer_post_def
+        prefix_diverge_post_def design_def expr_if_def rad_state.wait_def
+        SEXP_def lens_defs fun_eq_iff Let_def)
+    using assms
+    by (pred_auto; auto)
+  show ?thesis
+    apply (simp only: RAD_angelic_choice Prefix_Skip_RAD_RA
+        Prefix_Chaos_RAD_RA Prefix_Choice_RAD_RA RA_conj[symmetric])
+    by (simp only: design_eq)
+qed
+
+
+subsection \<open>Mapping examples (Examples 13-14)\<close>
+
+(* Paper Example 13: CSP Skip maps to the reactive angelic identity. *)
+lemma rad_p2ac_Skip_R:
+  "rad_p2ac (II\<^sub>C :: ('t::trace, 'e set) rp_hrel) = II_Rac"
+  by (rule rad_p2ac_II_C)
+
+definition prefix_offer_pair_post ::
+  "'e \<Rightarrow> 'e \<Rightarrow> ('e list, 'e) reactive_angelic_design" where
+[pred]: "prefix_offer_pair_post a b = (\<lambda> (s0, ac').
+  \<exists> y \<in> achoices.ac\<^sub>v (des_vars.more ac').
+    rad_state.wait\<^sub>v y \<and>
+    rad_state.tr\<^sub>v y =
+      rad_state.tr\<^sub>v (astate.s\<^sub>v (des_vars.more s0)) \<and>
+    a \<notin> rad_state.ref\<^sub>v y \<and> b \<notin> rad_state.ref\<^sub>v y)"
+
+(* The singleton round trip in Paper Example 14. *)
+lemma rad_p2ac_ac2p_prefix_stop_pair:
+  assumes "a \<noteq> b"
+  shows "(rad_p2ac \<circ> rad_ac2p)
+      (prefix_stop_post a \<and> prefix_stop_post b) =
+    prefix_offer_pair_post a b"
+  apply (simp only: rad_p2ac_ac2p)
+  apply (simp add: prefix_stop_post_def prefix_offer_pair_post_def
+      fun_eq_iff lens_defs des_vars.more\<^sub>L_def conj_pred_def)  using assms
+  apply (intro allI)
+  apply (rule iffI)
+   apply (elim exE conjE bexE)
+   subgoal premises assms for aa ba ac0 y ya yb
+   proof -
+     have ya_eq: "ya = y"
+       using assms(2,4) by auto
+     have yb_eq: "yb = y"
+       using assms(2,7) by auto
+     show ?thesis
+       using assms ya_eq yb_eq
+       by (rule_tac x=y in bexI; auto)
+   qed
+  apply (elim bexE conjE)
+  subgoal for aa ba y
+    apply (rule_tac x="{y}" in exI)
+    apply (rule conjI)
+     apply (rule_tac x=y in bexI; auto)
+    apply (rule conjI)
+     apply (rule_tac x=y in bexI; auto)
+    apply (rule_tac x=y in exI)
+    by auto
+  done
+
+
+subsection \<open>External choice with Stop (Example 19)\<close>
+
+(* Paper Example 19. *)
+(* Todo: this proof is very lengthy by chatgpt *)
+lemma Prefix_Chaos_Chaos_extchoice_Stop:
+  fixes a b :: 'e
+  shows
+  "((a \<rightarrow>\<^sub>R\<^sub>A\<^sub>D Chaos\<^sub>R\<^sub>A\<^sub>D)
+      \<squnion>\<^sub>R\<^sub>A\<^sub>D
+      (b \<rightarrow>\<^sub>R\<^sub>A\<^sub>D Chaos\<^sub>R\<^sub>A\<^sub>D))
+      \<box>\<^sub>R\<^sub>A\<^sub>D Stop\<^sub>R\<^sub>A\<^sub>D =
+    (RA \<circ> A)
+      ((\<not> (prefix_diverge_post a \<and> prefix_diverge_post b)) \<turnstile>
+        prefix_offer_pair_post a b)"
+proof -
+  have prefix_diverge_wf:
+      "((prefix_diverge_post x :: ('e list, 'e) reactive_angelic_design)
+        \<^sub>wf) = prefix_diverge_post x" for x :: 'e
+    by (simp add: prefix_diverge_post_def rad_wait_false_def fun_eq_iff
+        subst_app_def subst_upd_def subst_id_def SEXP_def lens_defs
+        alpha_defs)
+  have prefix_offer_wf:
+      "((prefix_offer_post x :: ('e list, 'e) reactive_angelic_design)
+        \<^sub>wf) = prefix_offer_post x" for x :: 'e
+    by (simp add: prefix_offer_post_def rad_wait_false_def fun_eq_iff
+        subst_app_def subst_upd_def subst_id_def SEXP_def lens_defs
+        alpha_defs)
+  have prefix_diverge_ok_out_subst:
+      "(prefix_diverge_post x)\<lbrakk>\<guillemotleft>c\<guillemotright>/ok\<^sup>>\<rbrakk> =
+        prefix_diverge_post x" for x :: 'e and c :: bool
+    by (simp add: prefix_diverge_post_def fun_eq_iff subst_app_def
+        subst_upd_def subst_id_def SEXP_def lens_defs des_vars.ok_def
+        astate.s_def des_vars.more\<^sub>L_def)
+  have prefix_offer_ok_out_subst:
+      "(prefix_offer_post x)\<lbrakk>\<guillemotleft>c\<guillemotright>/ok\<^sup>>\<rbrakk> =
+        prefix_offer_post x" for x :: 'e and c :: bool
+    by (simp add: prefix_offer_post_def fun_eq_iff subst_app_def
+        subst_upd_def subst_id_def SEXP_def lens_defs des_vars.ok_def
+        astate.s_def des_vars.more\<^sub>L_def)
+  note prefix_diverge_ok_out_subst[usubst]
+  note prefix_offer_ok_out_subst[usubst]
+  have chaos_absorb:
+      "(RA \<circ> A) ((\<not> prefix_diverge_post x) \<turnstile>
+          (prefix_offer_post x \<or> prefix_diverge_post x)) =
+       RA ((\<not> prefix_diverge_post x) \<turnstile>
+          (prefix_offer_post x \<or> prefix_diverge_post x))" for x :: 'e
+    by (rule RA_A_absorb_design)
+      (simp_all add: Healthy_def' PBMH_ades_disj unrest)
+  have branch_components:
+      "(((RA ((\<not> prefix_diverge_post x) \<turnstile>
+          (prefix_offer_post x \<or> prefix_diverge_post x)))
+          \<^sub>wf)\<^sup>f) =
+          RA2 (RA1 ((\<not> ok\<^sup><) \<or> prefix_diverge_post x)) \<and>
+       (((RA ((\<not> prefix_diverge_post x) \<turnstile>
+          (prefix_offer_post x \<or> prefix_diverge_post x)))
+          \<^sub>wf)\<^sup>t) =
+          RA2 (RA1 ((\<not> ok\<^sup><) \<or> prefix_diverge_post x \<or>
+            (prefix_offer_post x \<or> prefix_diverge_post x)))" for x :: 'e
+  proof -
+    let ?D = "prefix_diverge_post x"
+    let ?T = "prefix_offer_post x \<or> ?D"
+    let ?B = "?D \<or> (?T \<and> ok\<^sup>>)"
+    have B_wf: "(?B \<^sub>wf) = ?B"
+      by (simp only: rad_wait_false_disj rad_wait_false_conj
+          prefix_diverge_wf prefix_offer_wf rad_wait_false_ok_out)
+    have B_false: "?B\<^sup>f = ?D"
+      by (simp add: usubst usubst_eval; pred_auto)
+    have B_true: "?B\<^sup>t = ?T"
+      by (simp add: usubst usubst_eval; pred_auto)
+    have design_norm:
+        "((\<not> (?B \<^sub>wf)\<^sup>f) \<turnstile> (?B \<^sub>wf)\<^sup>t) =
+         ((\<not> ?D) \<turnstile> ?T)"
+      by (simp only: B_wf B_false B_true)
+    have false_component:
+        "((rad_wait_false \<circ> RA \<circ> A)
+          ((\<not> ?D) \<turnstile> ?T))\<^sup>f =
+         (RA2 \<circ> RA1 \<circ> PBMH_ades)
+          ((\<not> ok\<^sup><) \<or> (?B \<^sub>wf)\<^sup>f)"
+      using RA_design_wf_ok_false[of ?B]
+      by (simp only: design_norm)
+    have true_component:
+        "((rad_wait_false \<circ> RA \<circ> A)
+          ((\<not> ?D) \<turnstile> ?T))\<^sup>t =
+         (RA2 \<circ> RA1 \<circ> PBMH_ades)
+          ((\<not> ok\<^sup><) \<or> (?B \<^sub>wf)\<^sup>f \<or>
+            (?B \<^sub>wf)\<^sup>t)"
+      using RA_design_wf_ok_true[of ?B]
+      by (simp only: design_norm)
+    have absorb:
+        "RA (A ((\<not> ?D) \<turnstile> ?T)) = RA ((\<not> ?D) \<turnstile> ?T)"
+      using chaos_absorb[of x]
+      by (simp only: comp_apply)
+    show ?thesis
+      using false_component true_component
+      by (simp only: comp_apply absorb B_wf B_false B_true
+          PBMH_ades_disj PBMH_ades_not_ok_expr
+          prefix_diverge_post_PBMH prefix_offer_post_PBMH)
+  qed
+  have branch_false:
+      "(((RA ((\<not> prefix_diverge_post x) \<turnstile>
+          (prefix_offer_post x \<or> prefix_diverge_post x)))
+          \<^sub>wf)\<^sup>f) =
+        RA2 (RA1 ((\<not> ok\<^sup><) \<or> prefix_diverge_post x))" for x :: 'e
+    using branch_components[of x] by (rule conjunct1)
+  have branch_true:
+      "(((RA ((\<not> prefix_diverge_post x) \<turnstile>
+          (prefix_offer_post x \<or> prefix_diverge_post x)))
+          \<^sub>wf)\<^sup>t) =
+        RA2 (RA1 ((\<not> ok\<^sup><) \<or> prefix_diverge_post x \<or>
+          (prefix_offer_post x \<or> prefix_diverge_post x)))" for x :: 'e
+    using branch_components[of x] by (rule conjunct2)
+  have failure_conj:
+      "(RA2 (RA1 ((\<not> ok\<^sup><) \<or> prefix_diverge_post a)) \<and>
+        RA2 (RA1 ((\<not> ok\<^sup><) \<or> prefix_diverge_post b))) =
+       RA2 (RA1 ((\<not> ok\<^sup><) \<or>
+        (prefix_diverge_post a \<and> prefix_diverge_post b)))"
+    apply (simp only: RA2_conj[symmetric] RA1_conj[symmetric])
+    apply (rule arg_cong[where f=RA2])
+    apply (rule arg_cong[where f=RA1])
+    by pred_auto
+  have post_conj:
+      "(RA2 (RA1 ((\<not> ok\<^sup><) \<or> prefix_diverge_post a \<or>
+          (prefix_offer_post a \<or> prefix_diverge_post a))) \<and>
+        RA2 (RA1 ((\<not> ok\<^sup><) \<or> prefix_diverge_post b \<or>
+          (prefix_offer_post b \<or> prefix_diverge_post b)))) =
+       RA2 (RA1 ((\<not> ok\<^sup><) \<or>
+        (prefix_diverge_post a \<and> prefix_diverge_post b) \<or>
+        ((prefix_offer_post a \<or> prefix_diverge_post a) \<and>
+         (prefix_offer_post b \<or> prefix_diverge_post b))))"
+    apply (simp only: RA2_conj[symmetric] RA1_conj[symmetric])
+    apply (rule arg_cong[where f=RA2])
+    apply (rule arg_cong[where f=RA1])
+    by pred_auto
+  have prepend_inj:
+      "inj (rad_state.tr\<^sub>v_update ((+) (xs :: 'e list)) ::
+        ('e list, 'e) rad_state \<Rightarrow> ('e list, 'e) rad_state)" for xs
+    apply (rule injI)
+    subgoal for x y
+      by (cases x; cases y; simp;
+          rule left_cancel_monoid_class.add_left_imp_eq)
+    done
+  have prepend_eq:
+      "rad_state.tr\<^sub>v_update ((+) (xs :: 'e list)) x =
+       rad_state.tr\<^sub>v_update ((+) xs) y \<longleftrightarrow> x = y"
+      for xs and x y :: "('e list, 'e) rad_state"
+    by (rule inj_eq[OF prepend_inj])
+  note prepend_eq[simp]
+  have singleton_normalise:
+      "(\<lambda>x. RA2 (RA1
+          ((\<not> ok\<^sup><) \<or>
+           (prefix_diverge_post a \<and> prefix_diverge_post b))) x \<or>
+        (\<in>\<^sub>a\<^sub>c(RA2 (RA1
+          ((\<not> ok\<^sup><) \<or>
+           (prefix_diverge_post a \<and> prefix_diverge_post b) \<or>
+           ((prefix_offer_post a \<or> prefix_diverge_post a) \<and>
+            (prefix_offer_post b \<or> prefix_diverge_post b)))))) x) =
+       RA2 (RA1
+        ((\<not> ok\<^sup><) \<or>
+         (prefix_diverge_post a \<and> prefix_diverge_post b) \<or>
+         prefix_offer_pair_post a b))"
+    apply (simp add: ades_singleton_choice_def RA2_def RA1_def
+        prefix_diverge_post_def prefix_offer_post_def
+        prefix_offer_pair_post_def fun_eq_iff Let_def
+        rad_normalise_choices_as_prepend rad_zero_trace_def
+        rad_trace_extensions_def lens_defs des_vars.ok_def astate.s_def
+        des_vars.more\<^sub>L_def SEXP_def conj_pred_def disj_pred_def
+        not_pred_def)
+    apply (intro allI)
+    subgoal for aa ba
+      apply (cases "astate.s\<^sub>v (des_vars.more aa)")
+      apply (cases "des_vars.more aa")
+      apply (cases aa)
+      apply (cases "des_vars.more ba")
+      apply (cases ba)
+      apply (simp add: subst_app_def subst_ext_def ns_alpha_def
+          lens_comp_def fst_lens_def des_vars.ok_def SEXP_def)
+      apply auto
+      done
+    done
+  have pair_p2ac:
+      "prefix_offer_pair_post a b = p2ac \<lceil>(\<lambda> (s, y).
+        rad_state.wait\<^sub>v y \<and>
+        rad_state.tr\<^sub>v y = rad_state.tr\<^sub>v s \<and>
+        a \<notin> rad_state.ref\<^sub>v y \<and>
+        b \<notin> rad_state.ref\<^sub>v y)\<rceil>\<^sub>D"
+    by (simp add: prefix_offer_pair_post_def p2ac_def fun_eq_iff
+        subst_app_def subst_ext_def SEXP_def lens_defs
+        des_vars.more\<^sub>L_def; pred_auto; blast)
+  have pair_PBMH:
+      "PBMH_ades (prefix_offer_pair_post a b) =
+        prefix_offer_pair_post a b"
+    by (simp only: pair_p2ac PBMH_ades_p2ac)
+  have pair_unrest: "$ok\<^sup>> \<sharp> prefix_offer_pair_post a b"
+    apply (simp add: unrest_lens prefix_offer_pair_post_def)
+    apply (simp add: subst_app_def subst_upd_def subst_id_def
+        SEXP_def lens_defs alpha_defs)
+    done
+  let ?F = "prefix_diverge_post a \<and> prefix_diverge_post b"
+  let ?T = "(prefix_offer_post a \<or> prefix_diverge_post a) \<and>
+      (prefix_offer_post b \<or> prefix_diverge_post b)"
+  let ?R = "prefix_offer_pair_post a b"
+  let ?U = "RA2 (RA1 ((\<not> ok\<^sup><) \<or> ?F))"
+  let ?V = "RA2 (RA1 ((\<not> ok\<^sup><) \<or> ?F \<or> ?T))"
+  let ?S = "\<in>\<^sub>a\<^sub>c(?V)"
+  let ?W = "RA2 (RA1 ((\<not> ok\<^sup><) \<or> ?F \<or> ?R))"
+  have singleton_normalise': "(\<lambda>x. ?U x \<or> ?S x) = ?W"
+    using singleton_normalise .
+  have post_absorb:
+      "(?U \<or> (?S \<and> ok\<^sup>>)) = (?U \<or> (?W \<and> ok\<^sup>>))"
+  proof (rule ext)
+    fix x
+    have pointwise: "(?U x \<or> ?S x) = ?W x"
+      by (rule fun_cong[OF singleton_normalise'])
+    show "(?U \<or> (?S \<and> ok\<^sup>>)) x =
+        (?U \<or> (?W \<and> ok\<^sup>>)) x"
+      using pointwise
+      by (simp only: conj_pred_def disj_pred_def; blast)
+  qed
+  have design_eq: "((\<not> ?U) \<turnstile> ?S) = ((\<not> ?U) \<turnstile> ?W)"
+    by (simp only: design_as_disj pred_ba.double_compl
+        pred_ba.sup_assoc post_absorb)
+  have left_H: "((\<not> ?U) \<turnstile> ?S) is \<^bold>H"
+    by (rule design_is_H1_H2; simp add: unrest)
+  have right_H: "((\<not> ?F) \<turnstile> ?R) is \<^bold>H"
+    by (rule design_is_H1_H2; simp add: unrest pair_unrest)
+  have F_PBMH: "?F is PBMH_ades"
+    by (rule PBMH_ades_conj_closure; simp add: Healthy_def')
+  have X_PBMH: "PBMH_ades ((\<not> ok\<^sup><) \<or> ?F) =
+      ((\<not> ok\<^sup><) \<or> ?F)"
+    using F_PBMH by (simp add: PBMH_ades_disj Healthy_def')
+  have Z_PBMH: "PBMH_ades ((\<not> ok\<^sup><) \<or> ?F \<or> ?R) =
+      ((\<not> ok\<^sup><) \<or> ?F \<or> ?R)"
+    using F_PBMH pair_PBMH
+    by (simp add: PBMH_ades_disj Healthy_def')
+  have outer_normalise:
+      "(RA \<circ> A) ((\<not> ?U) \<turnstile> ?S) =
+       (RA \<circ> A) ((\<not> ?F) \<turnstile> ?R)"
+  proof -
+    have "(RA \<circ> A) ((\<not> ?U) \<turnstile> ?S) =
+        RA (PBMH_ades ((\<not> ?U) \<turnstile> ?S))"
+      by (simp only: comp_apply RA_A'[OF left_H])
+    also have "... = RA (PBMH_ades ((\<not> ?U) \<turnstile> ?W))"
+      by (simp only: design_eq)
+    also have "... = RA (PBMH_ades ((\<not> ?F) \<turnstile> ?R))"
+      using RA_design_PBMH_normalise[of ?F ?R]
+      by (simp only: X_PBMH Z_PBMH)
+    also have "... = (RA \<circ> A) ((\<not> ?F) \<turnstile> ?R)"
+      by (simp only: comp_apply RA_A'[OF right_H])
+    finally show ?thesis .
+  qed
+  show ?thesis
+    apply (subst extchoice_RAD_Stop)
+     apply (rule RAD_angelic_closure;
+         rule Prefix_RAD_closure;
+         rule Chaos_RAD_is_RAD)
+    apply (simp only: RAD_angelic_choice rad_wait_false_conj subst_pred
+        Prefix_Chaos_RAD_RA branch_false branch_true)
+    apply (simp only: failure_conj post_conj)
+    apply (subst ades_singleton_choice_def[symmetric])
+    by (rule outer_normalise)
 qed
 
 end
