utp_ap_ops.thy
@@ -1,0 +1,203 @@
+section \<open>Angelic Process Operators\<close>
+
+theory utp_ap_ops
+  imports utp_ap_rad
+begin
+
+subsection \<open>Angelic Choice\<close>
+
+abbreviation achoice_AP ::
+  "('t::trace, 'e) reactive_angelic_design \<Rightarrow> ('t, 'e) reactive_angelic_design \<Rightarrow>
+   ('t, 'e) reactive_angelic_design"
+  (infixl "\<squnion>\<^sub>A\<^sub>P" 70)
+where "P \<squnion>\<^sub>A\<^sub>P Q \<equiv> P \<squnion> Q"
+
+(* Paper Definition 50. *)
+lemma AP_angelic_choice:
+  "P \<squnion>\<^sub>A\<^sub>P Q = (P \<and> Q)"
+  by (simp add: conj_pred_def)
+
+(* Conjunction of two designs with negated preconditions. *)
+lemma design_neg_pre_conj:
+  "(((\<not> F1) \<turnstile> T1) \<and> ((\<not> F2) \<turnstile> T2)) =
+   ((\<not> (F1 \<and> F2)) \<turnstile>
+    ((F1 \<or> T1) \<and> (F2 \<or> T2)))"
+  by pred_auto
+
+(* The angelic choice of two angelic processes as the RA3AP image of
+   the conjoined normal-form design bodies. *)
+lemma AP_angelic_choice_form:
+  assumes "P is AP" "Q is AP"
+  shows "P \<squnion>\<^sub>A\<^sub>P Q =
+    RA3AP (((\<not> RA2 (PBMH_ades ((P \<^sub>wf)\<^sup>f))) \<turnstile>
+            RA2 (RA1 (PBMH_ades ((P \<^sub>wf)\<^sup>t)))) \<and>
+           ((\<not> RA2 (PBMH_ades ((Q \<^sub>wf)\<^sup>f))) \<turnstile>
+            RA2 (RA1 (PBMH_ades ((Q \<^sub>wf)\<^sup>t)))))"
+proof -
+  have "P \<squnion>\<^sub>A\<^sub>P Q = (AP P \<and> AP Q)"
+    by (simp only: AP_angelic_choice Healthy_if[OF assms(1)]
+        Healthy_if[OF assms(2)])
+  also have "... =
+      (RA3AP ((\<not> RA2 (PBMH_ades ((P \<^sub>wf)\<^sup>f))) \<turnstile>
+              RA2 (RA1 (PBMH_ades ((P \<^sub>wf)\<^sup>t)))) \<and>
+       RA3AP ((\<not> RA2 (PBMH_ades ((Q \<^sub>wf)\<^sup>f))) \<turnstile>
+              RA2 (RA1 (PBMH_ades ((Q \<^sub>wf)\<^sup>t)))))"
+    by (simp only: AP_RA3AP_design)
+  finally show ?thesis
+    by (simp only: RA3AP_conj[symmetric])
+qed
+
+(* The RA3AP design form of the angelic choice of two angelic
+   processes.  The postcondition disjuncts F \<or> T are the paper's
+   implications \<not> F \<longrightarrow> T. *)
+lemma AP_angelic_choice_design:
+  assumes "P is AP" "Q is AP"
+  shows "P \<squnion>\<^sub>A\<^sub>P Q =
+    RA3AP ((\<not> (RA2 (PBMH_ades ((P \<^sub>wf)\<^sup>f)) \<and>
+               RA2 (PBMH_ades ((Q \<^sub>wf)\<^sup>f)))) \<turnstile>
+           ((RA2 (PBMH_ades ((P \<^sub>wf)\<^sup>f)) \<or>
+             RA2 (RA1 (PBMH_ades ((P \<^sub>wf)\<^sup>t)))) \<and>
+            (RA2 (PBMH_ades ((Q \<^sub>wf)\<^sup>f)) \<or>
+             RA2 (RA1 (PBMH_ades ((Q \<^sub>wf)\<^sup>t))))))"
+  by (simp only: AP_angelic_choice_form[OF assms]
+      design_neg_pre_conj)
+
+(* Thesis Theorem T.6.4.1: angelic processes are closed under angelic
+   choice. *)
+lemma AP_angelic_closure [closure]:
+  assumes "P is AP" "Q is AP"
+  shows "P \<squnion>\<^sub>A\<^sub>P Q is AP"
+proof -
+  let ?NP = "((\<not> RA2 (PBMH_ades ((P \<^sub>wf)\<^sup>f))) \<turnstile>
+              RA2 (RA1 (PBMH_ades ((P \<^sub>wf)\<^sup>t))))"
+  let ?NQ = "((\<not> RA2 (PBMH_ades ((Q \<^sub>wf)\<^sup>f))) \<turnstile>
+              RA2 (RA1 (PBMH_ades ((Q \<^sub>wf)\<^sup>t))))"
+  have C_A: "(?NP \<and> ?NQ) is A"
+    using A_angelic_closure[OF AP_body_is_A[of P] AP_body_is_A[of Q]]
+    by (simp only: angelic_design_angelic)
+  have C_RA2: "(?NP \<and> ?NQ) is RA2"
+    by (rule Healthy_intro,
+        simp only: RA2_conj Healthy_if[OF AP_body_is_RA2])
+  show ?thesis
+    by (simp only: AP_angelic_choice_form[OF assms]
+        RA3AP_AP_closure[OF C_A C_RA2])
+qed
+
+subsection \<open>Choice\<close>
+
+(* Paper Definition 54. *)
+definition Choice_AP ::
+  "('t::trace, 'e) reactive_angelic_design" ("Choice\<^sub>A\<^sub>P") where
+[pred]: "Choice_AP = AP (true \<turnstile> ac_non_empty)"
+
+lemma Choice_AP_is_AP [closure]: "Choice\<^sub>A\<^sub>P is AP"
+  by (simp add: Choice_AP_def AP_healthy)
+
+lemmas Choice_AP_facts =
+  rad_wait_false_ac_non_empty PBMH_ades_ac_non_empty
+  ac_non_empty_ok_out_subst
+
+lemmas true_post_facts =
+  rad_wait_false_true PBMH_ades_true subst_pred(1)
+
+(* Thesis Lemma L.6.4.3: the design form of Choice_AP. *)
+lemma Choice_AP_design:
+  "Choice\<^sub>A\<^sub>P =
+   (true \<turnstile>
+    (ades_state_choice \<triangleleft> $rad_wait_lens\<^sup>< \<triangleright>
+     RA1 true))"
+  by (simp only: Choice_AP_def AP_true_design[OF Choice_AP_facts]
+      RA1_RA2_ac_non_empty)
+
+(* Choice_AP with the wait conditional folded back into RA3AP. *)
+lemma Choice_AP_RA3AP: "Choice\<^sub>A\<^sub>P = RA3AP (true \<turnstile> RA1 true)"
+  by (simp only: Choice_AP_design RA3AP_design expr_if_idem)
+
+(* The non-emptiness requirement is already enforced by AP. *)
+lemma Choice_AP_alt: "Choice\<^sub>A\<^sub>P = AP (true \<turnstile> true)"
+  by (simp only: Choice_AP_design
+      AP_true_design[OF true_post_facts] RA2_true)
+
+(* Paper Theorem 53 / Thesis Theorem T.6.4.12. *)
+theorem H1_Choice_RAD:
+  "H1 Choice\<^sub>R\<^sub>A\<^sub>D = Choice\<^sub>A\<^sub>P"
+  by (simp only: Choice_RAD_RA Choice_AP_alt
+      H1_RA_true_design[OF true_post_facts])
+
+(* Paper Theorem 54 / Thesis Theorem T.6.4.13. *)
+theorem RA1_Choice_AP:
+  "RA1 Choice\<^sub>A\<^sub>P = Choice\<^sub>R\<^sub>A\<^sub>D"
+  by (simp only: Choice_AP_alt Choice_RAD_RA
+      RA1_AP_true_design[OF true_post_facts])
+
+subsection \<open>Stop\<close>
+
+(* Paper Definition 55. *)
+definition Stop_AP ::
+  "('t::trace, 'e) reactive_angelic_design" ("Stop\<^sub>A\<^sub>P") where
+[pred]: "Stop_AP = AP (true \<turnstile> stop_post)"
+
+lemma Stop_AP_is_AP [closure]: "Stop\<^sub>A\<^sub>P is AP"
+  by (simp add: Stop_AP_def AP_healthy)
+
+lemmas Stop_AP_facts =
+  rad_wait_false_stop_post stop_post_PBMH stop_post_ok_out_subst
+
+(* The design form of Stop_AP: while waiting the state is unchanged,
+   and otherwise the Stop postcondition holds under RA1. *)
+lemma Stop_AP_design:
+  "Stop\<^sub>A\<^sub>P =
+   (true \<turnstile>
+    (ades_state_choice \<triangleleft> $rad_wait_lens\<^sup>< \<triangleright>
+     RA1 stop_post))"
+  by (simp only: Stop_AP_def AP_true_design[OF Stop_AP_facts]
+      RA2_stop_post)
+
+(* Paper Theorem 55 / Thesis Theorem T.6.4.14. *)
+theorem H1_Stop_RAD:
+  "H1 Stop\<^sub>R\<^sub>A\<^sub>D = Stop\<^sub>A\<^sub>P"
+  by (simp only: Stop_RAD_RA Stop_AP_def
+      H1_RA_true_design[OF Stop_AP_facts])
+
+(* Paper Theorem 56 / Thesis Theorem T.6.4.15. *)
+theorem RA1_Stop_AP:
+  "RA1 Stop\<^sub>A\<^sub>P = Stop\<^sub>R\<^sub>A\<^sub>D"
+  by (simp only: Stop_AP_def Stop_RAD_RA
+      RA1_AP_true_design[OF Stop_AP_facts])
+
+subsection \<open>Skip\<close>
+
+(* Paper Definition 56. *)
+definition Skip_AP ::
+  "('t::trace, 'e) reactive_angelic_design" ("Skip\<^sub>A\<^sub>P") where
+[pred]: "Skip_AP = AP (true \<turnstile> skip_post)"
+
+lemma Skip_AP_is_AP [closure]: "Skip\<^sub>A\<^sub>P is AP"
+  by (simp add: Skip_AP_def AP_healthy)
+
+lemmas Skip_AP_facts =
+  rad_wait_false_skip_post skip_post_PBMH skip_post_ok_out_subst
+
+(* The design form of Skip_AP: while waiting the state is unchanged,
+   and otherwise the Skip postcondition holds under RA1. *)
+lemma Skip_AP_design:
+  "Skip\<^sub>A\<^sub>P =
+   (true \<turnstile>
+    (ades_state_choice \<triangleleft> $rad_wait_lens\<^sup>< \<triangleright>
+     RA1 skip_post))"
+  by (simp only: Skip_AP_def AP_true_design[OF Skip_AP_facts]
+      RA2_skip_post)
+
+(* Paper Theorem 57 / Thesis Theorem T.6.4.16. *)
+theorem H1_Skip_RAD:
+  "H1 Skip\<^sub>R\<^sub>A\<^sub>D = Skip\<^sub>A\<^sub>P"
+  by (simp only: Skip_RAD_RA Skip_AP_def
+      H1_RA_true_design[OF Skip_AP_facts])
+
+(* Paper Theorem 58 / Thesis Theorem T.6.4.17. *)
+theorem RA1_Skip_AP:
+  "RA1 Skip\<^sub>A\<^sub>P = Skip\<^sub>R\<^sub>A\<^sub>D"
+  by (simp only: Skip_AP_def Skip_RAD_RA
+      RA1_AP_true_design[OF Skip_AP_facts])
+
+end
